src/lib/Pulse.Lib.BigStar.fsti
@@ -120,15 +120,13 @@ val fn bigstar_zs_elim
   ensures  emp
 ```
 
-```pulse
-ghost
-val fn bigstar_zs_intro
+val bigstar_zs_intro
   (#[exact (`0)] u1 : int)
   (m : nat)
   (f: (i: nat{m <= i /\ i < m} -> slprop))
-  requires emp
-  ensures  bigstar #u1 m m f
-```
+  : stt_ghost unit emp_inames
+      (requires emp)
+      (ensures  fun _ -> bigstar #u1 m m f)
 
 ```pulse
 ghost
@@ -140,15 +138,13 @@ val fn bigstar_single_elim
   ensures  f m
 ```
 
-```pulse
-ghost
-val fn bigstar_single_intro
+val bigstar_single_intro
   (#[exact (`0)] u1 : int)
   (m : nat)
   (f: (i: nat{m <= i /\ i < (m+1)} -> slprop))
-  requires f m
-  ensures  bigstar #u1 m (m+1) f
-```
+  : stt_ghost unit emp_inames
+      (requires f m)
+      (ensures  fun _ -> bigstar #u1 m (m+1) f)
 
 ```pulse
 ghost
